AwsCryptographicMaterialProviders/runtimes/net/Generated/AwsCryptographyKeyStore/NativeWrapper_KeyStorageInterface.cs
@@ -45,6 +45,34 @@ namespace AWS.Cryptography.KeyStore
     {
       throw new KeyStoreException("Not supported at this time.");
     }
+    public Wrappers_Compile._IResult<software.amazon.cryptography.keystore.internaldafny.types._IGetMutationOutput, software.amazon.cryptography.keystore.internaldafny.types._IError> GetMutation(software.amazon.cryptography.keystore.internaldafny.types._IGetMutationInput input)
+    {
+      void validateOutput(AWS.Cryptography.KeyStore.GetMutationOutput nativeOutput)
+      {
+        try { nativeOutput.Validate(); }
+        catch (ArgumentException e)
+        {
+          var message = $"Output of {_impl}._GetMutation is invalid. {e.Message}";
+          throw new KeyStoreException(message);
+        }
+      }
+      AWS.Cryptography.KeyStore.GetMutationInput nativeInput = TypeConversion.FromDafny_N3_aws__N12_cryptography__N8_keyStore__S16_GetMutationInput(input);
+      try
+      {
+        AWS.Cryptography.KeyStore.GetMutationOutput nativeOutput = _impl.GetMutation(nativeInput);
+        _ = nativeOutput ?? throw new KeyStoreException($"{_impl}._GetMutation returned null, should be {typeof(AWS.Cryptography.KeyStore.GetMutationOutput)}");
+        validateOutput(nativeOutput);
+        return Wrappers_Compile.Result<software.amazon.cryptography.keystore.internaldafny.types._IGetMutationOutput, software.amazon.cryptography.keystore.internaldafny.types._IError>.create_Success(TypeConversion.ToDafny_N3_aws__N12_cryptography__N8_keyStore__S17_GetMutationOutput(nativeOutput));
+      }
+      catch (Exception e)
+      {
+        return Wrappers_Compile.Result<software.amazon.cryptography.keystore.internaldafny.types._IGetMutationOutput, software.amazon.cryptography.keystore.internaldafny.types._IError>.create_Failure(TypeConversion.ToDafny_CommonError(e));
+      }
+    }
+    public Wrappers_Compile._IResult<software.amazon.cryptography.keystore.internaldafny.types._IGetMutationOutput, software.amazon.cryptography.keystore.internaldafny.types._IError> GetMutation_k(software.amazon.cryptography.keystore.internaldafny.types._IGetMutationInput input)
+    {
+      throw new KeyStoreException("Not supported at this time.");
+    }
     public Wrappers_Compile._IResult<software.amazon.cryptography.keystore.internaldafny.types._IGetItemsForInitializeMutationOutput, software.amazon.cryptography.keystore.internaldafny.types._IError> GetItemsForInitializeMutation(software.amazon.cryptography.keystore.internaldafny.types._IGetItemsForInitializeMutationInput input)
     {
       void validateOutput(AWS.Cryptography.KeyStore.GetItemsForInitializeMutationOutput nativeOutput)
@@ -70,34 +98,6 @@ namespace AWS.Cryptography.KeyStore
       }
     }
     public Wrappers_Compile._IResult<software.amazon.cryptography.keystore.internaldafny.types._IGetItemsForInitializeMutationOutput, software.amazon.cryptography.keystore.internaldafny.types._IError> GetItemsForInitializeMutation_k(software.amazon.cryptography.keystore.internaldafny.types._IGetItemsForInitializeMutationInput input)
-    {
-      throw new KeyStoreException("Not supported at this time.");
-    }
-    public Wrappers_Compile._IResult<software.amazon.cryptography.keystore.internaldafny.types._IGetMutationLockOutput, software.amazon.cryptography.keystore.internaldafny.types._IError> GetMutationLock(software.amazon.cryptography.keystore.internaldafny.types._IGetMutationLockInput input)
-    {
-      void validateOutput(AWS.Cryptography.KeyStore.GetMutationLockOutput nativeOutput)
-      {
-        try { nativeOutput.Validate(); }
-        catch (ArgumentException e)
-        {
-          var message = $"Output of {_impl}._GetMutationLock is invalid. {e.Message}";
-          throw new KeyStoreException(message);
-        }
-      }
-      AWS.Cryptography.KeyStore.GetMutationLockInput nativeInput = TypeConversion.FromDafny_N3_aws__N12_cryptography__N8_keyStore__S20_GetMutationLockInput(input);
-      try
-      {
-        AWS.Cryptography.KeyStore.GetMutationLockOutput nativeOutput = _impl.GetMutationLock(nativeInput);
-        _ = nativeOutput ?? throw new KeyStoreException($"{_impl}._GetMutationLock returned null, should be {typeof(AWS.Cryptography.KeyStore.GetMutationLockOutput)}");
-        validateOutput(nativeOutput);
-        return Wrappers_Compile.Result<software.amazon.cryptography.keystore.internaldafny.types._IGetMutationLockOutput, software.amazon.cryptography.keystore.internaldafny.types._IError>.create_Success(TypeConversion.ToDafny_N3_aws__N12_cryptography__N8_keyStore__S21_GetMutationLockOutput(nativeOutput));
-      }
-      catch (Exception e)
-      {
-        return Wrappers_Compile.Result<software.amazon.cryptography.keystore.internaldafny.types._IGetMutationLockOutput, software.amazon.cryptography.keystore.internaldafny.types._IError>.create_Failure(TypeConversion.ToDafny_CommonError(e));
-      }
-    }
-    public Wrappers_Compile._IResult<software.amazon.cryptography.keystore.internaldafny.types._IGetMutationLockOutput, software.amazon.cryptography.keystore.internaldafny.types._IError> GetMutationLock_k(software.amazon.cryptography.keystore.internaldafny.types._IGetMutationLockInput input)
     {
       throw new KeyStoreException("Not supported at this time.");
     }
@@ -157,31 +157,31 @@ namespace AWS.Cryptography.KeyStore
     {
       throw new KeyStoreException("Not supported at this time.");
     }
-    public Wrappers_Compile._IResult<software.amazon.cryptography.keystore.internaldafny.types._IDeleteMutationLockAndIndexOutput, software.amazon.cryptography.keystore.internaldafny.types._IError> DeleteMutationLockAndIndex(software.amazon.cryptography.keystore.internaldafny.types._IDeleteMutationLockAndIndexInput input)
+    public Wrappers_Compile._IResult<software.amazon.cryptography.keystore.internaldafny.types._IWriteAtomicMutationOutput, software.amazon.cryptography.keystore.internaldafny.types._IError> WriteAtomicMutation(software.amazon.cryptography.keystore.internaldafny.types._IWriteAtomicMutationInput input)
     {
-      void validateOutput(AWS.Cryptography.KeyStore.DeleteMutationLockAndIndexOutput nativeOutput)
+      void validateOutput(AWS.Cryptography.KeyStore.WriteAtomicMutationOutput nativeOutput)
       {
         try { nativeOutput.Validate(); }
         catch (ArgumentException e)
         {
-          var message = $"Output of {_impl}._DeleteMutationLockAndIndex is invalid. {e.Message}";
+          var message = $"Output of {_impl}._WriteAtomicMutation is invalid. {e.Message}";
           throw new KeyStoreException(message);
         }
       }
-      AWS.Cryptography.KeyStore.DeleteMutationLockAndIndexInput nativeInput = TypeConversion.FromDafny_N3_aws__N12_cryptography__N8_keyStore__S31_DeleteMutationLockAndIndexInput(input);
+      AWS.Cryptography.KeyStore.WriteAtomicMutationInput nativeInput = TypeConversion.FromDafny_N3_aws__N12_cryptography__N8_keyStore__S24_WriteAtomicMutationInput(input);
       try
       {
-        AWS.Cryptography.KeyStore.DeleteMutationLockAndIndexOutput nativeOutput = _impl.DeleteMutationLockAndIndex(nativeInput);
-        _ = nativeOutput ?? throw new KeyStoreException($"{_impl}._DeleteMutationLockAndIndex returned null, should be {typeof(AWS.Cryptography.KeyStore.DeleteMutationLockAndIndexOutput)}");
+        AWS.Cryptography.KeyStore.WriteAtomicMutationOutput nativeOutput = _impl.WriteAtomicMutation(nativeInput);
+        _ = nativeOutput ?? throw new KeyStoreException($"{_impl}._WriteAtomicMutation returned null, should be {typeof(AWS.Cryptography.KeyStore.WriteAtomicMutationOutput)}");
         validateOutput(nativeOutput);
-        return Wrappers_Compile.Result<software.amazon.cryptography.keystore.internaldafny.types._IDeleteMutationLockAndIndexOutput, software.amazon.cryptography.keystore.internaldafny.types._IError>.create_Success(TypeConversion.ToDafny_N3_aws__N12_cryptography__N8_keyStore__S32_DeleteMutationLockAndIndexOutput(nativeOutput));
+        return Wrappers_Compile.Result<software.amazon.cryptography.keystore.internaldafny.types._IWriteAtomicMutationOutput, software.amazon.cryptography.keystore.internaldafny.types._IError>.create_Success(TypeConversion.ToDafny_N3_aws__N12_cryptography__N8_keyStore__S25_WriteAtomicMutationOutput(nativeOutput));
       }
       catch (Exception e)
       {
-        return Wrappers_Compile.Result<software.amazon.cryptography.keystore.internaldafny.types._IDeleteMutationLockAndIndexOutput, software.amazon.cryptography.keystore.internaldafny.types._IError>.create_Failure(TypeConversion.ToDafny_CommonError(e));
+        return Wrappers_Compile.Result<software.amazon.cryptography.keystore.internaldafny.types._IWriteAtomicMutationOutput, software.amazon.cryptography.keystore.internaldafny.types._IError>.create_Failure(TypeConversion.ToDafny_CommonError(e));
       }
     }
-    public Wrappers_Compile._IResult<software.amazon.cryptography.keystore.internaldafny.types._IDeleteMutationLockAndIndexOutput, software.amazon.cryptography.keystore.internaldafny.types._IError> DeleteMutationLockAndIndex_k(software.amazon.cryptography.keystore.internaldafny.types._IDeleteMutationLockAndIndexInput input)
+    public Wrappers_Compile._IResult<software.amazon.cryptography.keystore.internaldafny.types._IWriteAtomicMutationOutput, software.amazon.cryptography.keystore.internaldafny.types._IError> WriteAtomicMutation_k(software.amazon.cryptography.keystore.internaldafny.types._IWriteAtomicMutationInput input)
     {
       throw new KeyStoreException("Not supported at this time.");
     }
@@ -325,34 +325,6 @@ namespace AWS.Cryptography.KeyStore
     {
       throw new KeyStoreException("Not supported at this time.");
     }
-    public Wrappers_Compile._IResult<software.amazon.cryptography.keystore.internaldafny.types._IGetMutationLockAndIndexOutput, software.amazon.cryptography.keystore.internaldafny.types._IError> GetMutationLockAndIndex(software.amazon.cryptography.keystore.internaldafny.types._IGetMutationLockAndIndexInput input)
-    {
-      void validateOutput(AWS.Cryptography.KeyStore.GetMutationLockAndIndexOutput nativeOutput)
-      {
-        try { nativeOutput.Validate(); }
-        catch (ArgumentException e)
-        {
-          var message = $"Output of {_impl}._GetMutationLockAndIndex is invalid. {e.Message}";
-          throw new KeyStoreException(message);
-        }
-      }
-      AWS.Cryptography.KeyStore.GetMutationLockAndIndexInput nativeInput = TypeConversion.FromDafny_N3_aws__N12_cryptography__N8_keyStore__S28_GetMutationLockAndIndexInput(input);
-      try
-      {
-        AWS.Cryptography.KeyStore.GetMutationLockAndIndexOutput nativeOutput = _impl.GetMutationLockAndIndex(nativeInput);
-        _ = nativeOutput ?? throw new KeyStoreException($"{_impl}._GetMutationLockAndIndex returned null, should be {typeof(AWS.Cryptography.KeyStore.GetMutationLockAndIndexOutput)}");
-        validateOutput(nativeOutput);
-        return Wrappers_Compile.Result<software.amazon.cryptography.keystore.internaldafny.types._IGetMutationLockAndIndexOutput, software.amazon.cryptography.keystore.internaldafny.types._IError>.create_Success(TypeConversion.ToDafny_N3_aws__N12_cryptography__N8_keyStore__S29_GetMutationLockAndIndexOutput(nativeOutput));
-      }
-      catch (Exception e)
-      {
-        return Wrappers_Compile.Result<software.amazon.cryptography.keystore.internaldafny.types._IGetMutationLockAndIndexOutput, software.amazon.cryptography.keystore.internaldafny.types._IError>.create_Failure(TypeConversion.ToDafny_CommonError(e));
-      }
-    }
-    public Wrappers_Compile._IResult<software.amazon.cryptography.keystore.internaldafny.types._IGetMutationLockAndIndexOutput, software.amazon.cryptography.keystore.internaldafny.types._IError> GetMutationLockAndIndex_k(software.amazon.cryptography.keystore.internaldafny.types._IGetMutationLockAndIndexInput input)
-    {
-      throw new KeyStoreException("Not supported at this time.");
-    }
     public Wrappers_Compile._IResult<software.amazon.cryptography.keystore.internaldafny.types._IQueryForVersionsOutput, software.amazon.cryptography.keystore.internaldafny.types._IError> QueryForVersions(software.amazon.cryptography.keystore.internaldafny.types._IQueryForVersionsInput input)
     {
       void validateOutput(AWS.Cryptography.KeyStore.QueryForVersionsOutput nativeOutput)
@@ -381,31 +353,31 @@ namespace AWS.Cryptography.KeyStore
     {
       throw new KeyStoreException("Not supported at this time.");
     }
-    public Wrappers_Compile._IResult<software.amazon.cryptography.keystore.internaldafny.types._IUpdateMutationIndexOutput, software.amazon.cryptography.keystore.internaldafny.types._IError> UpdateMutationIndex(software.amazon.cryptography.keystore.internaldafny.types._IUpdateMutationIndexInput input)
+    public Wrappers_Compile._IResult<software.amazon.cryptography.keystore.internaldafny.types._IDeleteMutationOutput, software.amazon.cryptography.keystore.internaldafny.types._IError> DeleteMutation(software.amazon.cryptography.keystore.internaldafny.types._IDeleteMutationInput input)
     {
-      void validateOutput(AWS.Cryptography.KeyStore.UpdateMutationIndexOutput nativeOutput)
+      void validateOutput(AWS.Cryptography.KeyStore.DeleteMutationOutput nativeOutput)
       {
         try { nativeOutput.Validate(); }
         catch (ArgumentException e)
         {
-          var message = $"Output of {_impl}._UpdateMutationIndex is invalid. {e.Message}";
+          var message = $"Output of {_impl}._DeleteMutation is invalid. {e.Message}";
           throw new KeyStoreException(message);
         }
       }
-      AWS.Cryptography.KeyStore.UpdateMutationIndexInput nativeInput = TypeConversion.FromDafny_N3_aws__N12_cryptography__N8_keyStore__S24_UpdateMutationIndexInput(input);
+      AWS.Cryptography.KeyStore.DeleteMutationInput nativeInput = TypeConversion.FromDafny_N3_aws__N12_cryptography__N8_keyStore__S19_DeleteMutationInput(input);
       try
       {
-        AWS.Cryptography.KeyStore.UpdateMutationIndexOutput nativeOutput = _impl.UpdateMutationIndex(nativeInput);
-        _ = nativeOutput ?? throw new KeyStoreException($"{_impl}._UpdateMutationIndex returned null, should be {typeof(AWS.Cryptography.KeyStore.UpdateMutationIndexOutput)}");
+        AWS.Cryptography.KeyStore.DeleteMutationOutput nativeOutput = _impl.DeleteMutation(nativeInput);
+        _ = nativeOutput ?? throw new KeyStoreException($"{_impl}._DeleteMutation returned null, should be {typeof(AWS.Cryptography.KeyStore.DeleteMutationOutput)}");
         validateOutput(nativeOutput);
-        return Wrappers_Compile.Result<software.amazon.cryptography.keystore.internaldafny.types._IUpdateMutationIndexOutput, software.amazon.cryptography.keystore.internaldafny.types._IError>.create_Success(TypeConversion.ToDafny_N3_aws__N12_cryptography__N8_keyStore__S25_UpdateMutationIndexOutput(nativeOutput));
+        return Wrappers_Compile.Result<software.amazon.cryptography.keystore.internaldafny.types._IDeleteMutationOutput, software.amazon.cryptography.keystore.internaldafny.types._IError>.create_Success(TypeConversion.ToDafny_N3_aws__N12_cryptography__N8_keyStore__S20_DeleteMutationOutput(nativeOutput));
       }
       catch (Exception e)
       {
-        return Wrappers_Compile.Result<software.amazon.cryptography.keystore.internaldafny.types._IUpdateMutationIndexOutput, software.amazon.cryptography.keystore.internaldafny.types._IError>.create_Failure(TypeConversion.ToDafny_CommonError(e));
+        return Wrappers_Compile.Result<software.amazon.cryptography.keystore.internaldafny.types._IDeleteMutationOutput, software.amazon.cryptography.keystore.internaldafny.types._IError>.create_Failure(TypeConversion.ToDafny_CommonError(e));
       }
     }
-    public Wrappers_Compile._IResult<software.amazon.cryptography.keystore.internaldafny.types._IUpdateMutationIndexOutput, software.amazon.cryptography.keystore.internaldafny.types._IError> UpdateMutationIndex_k(software.amazon.cryptography.keystore.internaldafny.types._IUpdateMutationIndexInput input)
+    public Wrappers_Compile._IResult<software.amazon.cryptography.keystore.internaldafny.types._IDeleteMutationOutput, software.amazon.cryptography.keystore.internaldafny.types._IError> DeleteMutation_k(software.amazon.cryptography.keystore.internaldafny.types._IDeleteMutationInput input)
     {
       throw new KeyStoreException("Not supported at this time.");
     }
