AwsCryptographicMaterialProviders/runtimes/net/Generated/AwsCryptographyKeyStore/WriteMutatedVersionsInput.cs
@@ -8,7 +8,9 @@ namespace AWS.Cryptography.KeyStore
   public class WriteMutatedVersionsInput
   {
     private System.Collections.Generic.List<AWS.Cryptography.KeyStore.OverWriteEncryptedHierarchicalKey> _items;
-    private AWS.Cryptography.KeyStore.MutationLock _mutationLock;
+    private AWS.Cryptography.KeyStore.MutationCommitment _mutationCommitment;
+    private AWS.Cryptography.KeyStore.OverWriteMutationIndex _mutationIndex;
+    private bool? _endMutation;
     public System.Collections.Generic.List<AWS.Cryptography.KeyStore.OverWriteEncryptedHierarchicalKey> Items
     {
       get { return this._items; }
@@ -18,19 +20,39 @@ namespace AWS.Cryptography.KeyStore
     {
       return this._items != null;
     }
-    public AWS.Cryptography.KeyStore.MutationLock MutationLock
+    public AWS.Cryptography.KeyStore.MutationCommitment MutationCommitment
     {
-      get { return this._mutationLock; }
-      set { this._mutationLock = value; }
+      get { return this._mutationCommitment; }
+      set { this._mutationCommitment = value; }
     }
-    public bool IsSetMutationLock()
+    public bool IsSetMutationCommitment()
     {
-      return this._mutationLock != null;
+      return this._mutationCommitment != null;
+    }
+    public AWS.Cryptography.KeyStore.OverWriteMutationIndex MutationIndex
+    {
+      get { return this._mutationIndex; }
+      set { this._mutationIndex = value; }
+    }
+    public bool IsSetMutationIndex()
+    {
+      return this._mutationIndex != null;
+    }
+    public bool EndMutation
+    {
+      get { return this._endMutation.GetValueOrDefault(); }
+      set { this._endMutation = value; }
+    }
+    public bool IsSetEndMutation()
+    {
+      return this._endMutation.HasValue;
     }
     public void Validate()
     {
       if (!IsSetItems()) throw new System.ArgumentException("Missing value for required property 'Items'");
-      if (!IsSetMutationLock()) throw new System.ArgumentException("Missing value for required property 'MutationLock'");
+      if (!IsSetMutationCommitment()) throw new System.ArgumentException("Missing value for required property 'MutationCommitment'");
+      if (!IsSetMutationIndex()) throw new System.ArgumentException("Missing value for required property 'MutationIndex'");
+      if (!IsSetEndMutation()) throw new System.ArgumentException("Missing value for required property 'EndMutation'");
 
     }
   }
