AwsCryptographicMaterialProviders/runtimes/python/src/aws_cryptographic_materialproviders/smithygenerated/aws_cryptography_keystore/dafny_to_smithy.py
@@ -210,8 +210,8 @@ def aws_cryptography_keystore_GetItemsForInitializeMutationInput(dafny_input):
     )
 
 
-def aws_cryptography_keystore_MutationLock(dafny_input):
-    return aws_cryptographic_materialproviders.smithygenerated.aws_cryptography_keystore.models.MutationLock(
+def aws_cryptography_keystore_MutationCommitment(dafny_input):
+    return aws_cryptographic_materialproviders.smithygenerated.aws_cryptography_keystore.models.MutationCommitment(
         identifier=b"".join(
             ord(c).to_bytes(2, "big") for c in dafny_input.Identifier
         ).decode("utf-16-be"),
@@ -223,6 +223,7 @@ def aws_cryptography_keystore_MutationLock(dafny_input):
         ),
         original=bytes(dafny_input.Original),
         terminal=bytes(dafny_input.Terminal),
+        input=bytes(dafny_input.Input),
         ciphertext_blob=bytes(dafny_input.CiphertextBlob),
     )
 
@@ -251,13 +252,13 @@ def aws_cryptography_keystore_GetItemsForInitializeMutationOutput(dafny_input):
         beacon_item=aws_cryptographic_materialproviders.smithygenerated.aws_cryptography_keystore.dafny_to_smithy.aws_cryptography_keystore_EncryptedHierarchicalKey(
             dafny_input.BeaconItem
         ),
-        mutation_lock=(
+        mutation_commitment=(
             (
-                aws_cryptographic_materialproviders.smithygenerated.aws_cryptography_keystore.dafny_to_smithy.aws_cryptography_keystore_MutationLock(
-                    dafny_input.MutationLock.value
+                aws_cryptographic_materialproviders.smithygenerated.aws_cryptography_keystore.dafny_to_smithy.aws_cryptography_keystore_MutationCommitment(
+                    dafny_input.MutationCommitment.value
                 )
             )
-            if (dafny_input.MutationLock.is_Some)
+            if (dafny_input.MutationCommitment.is_Some)
             else None
         ),
         mutation_index=(
@@ -274,17 +275,29 @@ def aws_cryptography_keystore_GetItemsForInitializeMutationOutput(dafny_input):
 
 def aws_cryptography_keystore_WriteInitializeMutationInput(dafny_input):
     return aws_cryptographic_materialproviders.smithygenerated.aws_cryptography_keystore.models.WriteInitializeMutationInput(
-        active=aws_cryptographic_materialproviders.smithygenerated.aws_cryptography_keystore.dafny_to_smithy.aws_cryptography_keystore_OverWriteEncryptedHierarchicalKey(
-            dafny_input.Active
+        active=(
+            (
+                aws_cryptographic_materialproviders.smithygenerated.aws_cryptography_keystore.dafny_to_smithy.aws_cryptography_keystore_OverWriteEncryptedHierarchicalKey(
+                    dafny_input.Active.value
+                )
+            )
+            if (dafny_input.Active.is_Some)
+            else None
         ),
-        version=aws_cryptographic_materialproviders.smithygenerated.aws_cryptography_keystore.dafny_to_smithy.aws_cryptography_keystore_EncryptedHierarchicalKey(
-            dafny_input.Version
+        version=(
+            (
+                aws_cryptographic_materialproviders.smithygenerated.aws_cryptography_keystore.dafny_to_smithy.aws_cryptography_keystore_EncryptedHierarchicalKey(
+                    dafny_input.Version.value
+                )
+            )
+            if (dafny_input.Version.is_Some)
+            else None
         ),
         beacon=aws_cryptographic_materialproviders.smithygenerated.aws_cryptography_keystore.dafny_to_smithy.aws_cryptography_keystore_OverWriteEncryptedHierarchicalKey(
             dafny_input.Beacon
         ),
-        mutation_lock=aws_cryptographic_materialproviders.smithygenerated.aws_cryptography_keystore.dafny_to_smithy.aws_cryptography_keystore_MutationLock(
-            dafny_input.MutationLock
+        mutation_commitment=aws_cryptographic_materialproviders.smithygenerated.aws_cryptography_keystore.dafny_to_smithy.aws_cryptography_keystore_MutationCommitment(
+            dafny_input.MutationCommitment
         ),
         mutation_index=aws_cryptographic_materialproviders.smithygenerated.aws_cryptography_keystore.dafny_to_smithy.aws_cryptography_keystore_MutationIndex(
             dafny_input.MutationIndex
@@ -295,6 +308,44 @@ def aws_cryptography_keystore_WriteInitializeMutationInput(dafny_input):
 def aws_cryptography_keystore_WriteInitializeMutationOutput(dafny_input):
     return (
         aws_cryptographic_materialproviders.smithygenerated.aws_cryptography_keystore.models.WriteInitializeMutationOutput()
+    )
+
+
+def aws_cryptography_keystore_WriteAtomicMutationInput(dafny_input):
+    return aws_cryptographic_materialproviders.smithygenerated.aws_cryptography_keystore.models.WriteAtomicMutationInput(
+        active=(
+            (
+                aws_cryptographic_materialproviders.smithygenerated.aws_cryptography_keystore.dafny_to_smithy.aws_cryptography_keystore_OverWriteEncryptedHierarchicalKey(
+                    dafny_input.Active.value
+                )
+            )
+            if (dafny_input.Active.is_Some)
+            else None
+        ),
+        version=(
+            (
+                aws_cryptographic_materialproviders.smithygenerated.aws_cryptography_keystore.dafny_to_smithy.aws_cryptography_keystore_EncryptedHierarchicalKey(
+                    dafny_input.Version.value
+                )
+            )
+            if (dafny_input.Version.is_Some)
+            else None
+        ),
+        beacon=aws_cryptographic_materialproviders.smithygenerated.aws_cryptography_keystore.dafny_to_smithy.aws_cryptography_keystore_OverWriteEncryptedHierarchicalKey(
+            dafny_input.Beacon
+        ),
+        items=[
+            aws_cryptographic_materialproviders.smithygenerated.aws_cryptography_keystore.dafny_to_smithy.aws_cryptography_keystore_OverWriteEncryptedHierarchicalKey(
+                list_element
+            )
+            for list_element in dafny_input.Items
+        ],
+    )
+
+
+def aws_cryptography_keystore_WriteAtomicMutationOutput(dafny_input):
+    return (
+        aws_cryptographic_materialproviders.smithygenerated.aws_cryptography_keystore.models.WriteAtomicMutationOutput()
     )
 
 
@@ -324,6 +375,17 @@ def aws_cryptography_keystore_QueryForVersionsOutput(dafny_input):
     )
 
 
+def aws_cryptography_keystore_OverWriteMutationIndex(dafny_input):
+    return aws_cryptographic_materialproviders.smithygenerated.aws_cryptography_keystore.models.OverWriteMutationIndex(
+        index=aws_cryptographic_materialproviders.smithygenerated.aws_cryptography_keystore.dafny_to_smithy.aws_cryptography_keystore_MutationIndex(
+            dafny_input.Index
+        ),
+        old=aws_cryptographic_materialproviders.smithygenerated.aws_cryptography_keystore.dafny_to_smithy.aws_cryptography_keystore_MutationIndex(
+            dafny_input.Old
+        ),
+    )
+
+
 def aws_cryptography_keystore_WriteMutatedVersionsInput(dafny_input):
     return aws_cryptographic_materialproviders.smithygenerated.aws_cryptography_keystore.models.WriteMutatedVersionsInput(
         items=[
@@ -332,9 +394,13 @@ def aws_cryptography_keystore_WriteMutatedVersionsInput(dafny_input):
             )
             for list_element in dafny_input.Items
         ],
-        mutation_lock=aws_cryptographic_materialproviders.smithygenerated.aws_cryptography_keystore.dafny_to_smithy.aws_cryptography_keystore_MutationLock(
-            dafny_input.MutationLock
+        mutation_commitment=aws_cryptographic_materialproviders.smithygenerated.aws_cryptography_keystore.dafny_to_smithy.aws_cryptography_keystore_MutationCommitment(
+            dafny_input.MutationCommitment
         ),
+        mutation_index=aws_cryptographic_materialproviders.smithygenerated.aws_cryptography_keystore.dafny_to_smithy.aws_cryptography_keystore_OverWriteMutationIndex(
+            dafny_input.MutationIndex
+        ),
+        end_mutation=dafny_input.EndMutation,
     )
 
 
@@ -344,62 +410,23 @@ def aws_cryptography_keystore_WriteMutatedVersionsOutput(dafny_input):
     )
 
 
-def aws_cryptography_keystore_UpdateMutationIndexInput(dafny_input):
-    return aws_cryptographic_materialproviders.smithygenerated.aws_cryptography_keystore.models.UpdateMutationIndexInput(
-        mutation_index=aws_cryptographic_materialproviders.smithygenerated.aws_cryptography_keystore.dafny_to_smithy.aws_cryptography_keystore_MutationIndex(
-            dafny_input.MutationIndex
-        ),
-        old_mutation_index=aws_cryptographic_materialproviders.smithygenerated.aws_cryptography_keystore.dafny_to_smithy.aws_cryptography_keystore_MutationIndex(
-            dafny_input.OldMutationIndex
-        ),
-    )
-
-
-def aws_cryptography_keystore_UpdateMutationIndexOutput(dafny_input):
-    return (
-        aws_cryptographic_materialproviders.smithygenerated.aws_cryptography_keystore.models.UpdateMutationIndexOutput()
-    )
-
-
-def aws_cryptography_keystore_GetMutationLockInput(dafny_input):
-    return aws_cryptographic_materialproviders.smithygenerated.aws_cryptography_keystore.models.GetMutationLockInput(
+def aws_cryptography_keystore_GetMutationInput(dafny_input):
+    return aws_cryptographic_materialproviders.smithygenerated.aws_cryptography_keystore.models.GetMutationInput(
         identifier=b"".join(
             ord(c).to_bytes(2, "big") for c in dafny_input.Identifier
         ).decode("utf-16-be"),
     )
 
 
-def aws_cryptography_keystore_GetMutationLockOutput(dafny_input):
-    return aws_cryptographic_materialproviders.smithygenerated.aws_cryptography_keystore.models.GetMutationLockOutput(
-        mutation_lock=(
+def aws_cryptography_keystore_GetMutationOutput(dafny_input):
+    return aws_cryptographic_materialproviders.smithygenerated.aws_cryptography_keystore.models.GetMutationOutput(
+        mutation_commitment=(
             (
-                aws_cryptographic_materialproviders.smithygenerated.aws_cryptography_keystore.dafny_to_smithy.aws_cryptography_keystore_MutationLock(
-                    dafny_input.MutationLock.value
+                aws_cryptographic_materialproviders.smithygenerated.aws_cryptography_keystore.dafny_to_smithy.aws_cryptography_keystore_MutationCommitment(
+                    dafny_input.MutationCommitment.value
                 )
             )
-            if (dafny_input.MutationLock.is_Some)
-            else None
-        ),
-    )
-
-
-def aws_cryptography_keystore_GetMutationLockAndIndexInput(dafny_input):
-    return aws_cryptographic_materialproviders.smithygenerated.aws_cryptography_keystore.models.GetMutationLockAndIndexInput(
-        identifier=b"".join(
-            ord(c).to_bytes(2, "big") for c in dafny_input.Identifier
-        ).decode("utf-16-be"),
-    )
-
-
-def aws_cryptography_keystore_GetMutationLockAndIndexOutput(dafny_input):
-    return aws_cryptographic_materialproviders.smithygenerated.aws_cryptography_keystore.models.GetMutationLockAndIndexOutput(
-        mutation_lock=(
-            (
-                aws_cryptographic_materialproviders.smithygenerated.aws_cryptography_keystore.dafny_to_smithy.aws_cryptography_keystore_MutationLock(
-                    dafny_input.MutationLock.value
-                )
-            )
-            if (dafny_input.MutationLock.is_Some)
+            if (dafny_input.MutationCommitment.is_Some)
             else None
         ),
         mutation_index=(
@@ -414,17 +441,17 @@ def aws_cryptography_keystore_GetMutationLockAndIndexOutput(dafny_input):
     )
 
 
-def aws_cryptography_keystore_DeleteMutationLockAndIndexInput(dafny_input):
-    return aws_cryptographic_materialproviders.smithygenerated.aws_cryptography_keystore.models.DeleteMutationLockAndIndexInput(
-        mutation_lock=aws_cryptographic_materialproviders.smithygenerated.aws_cryptography_keystore.dafny_to_smithy.aws_cryptography_keystore_MutationLock(
-            dafny_input.MutationLock
+def aws_cryptography_keystore_DeleteMutationInput(dafny_input):
+    return aws_cryptographic_materialproviders.smithygenerated.aws_cryptography_keystore.models.DeleteMutationInput(
+        mutation_commitment=aws_cryptographic_materialproviders.smithygenerated.aws_cryptography_keystore.dafny_to_smithy.aws_cryptography_keystore_MutationCommitment(
+            dafny_input.MutationCommitment
         ),
     )
 
 
-def aws_cryptography_keystore_DeleteMutationLockAndIndexOutput(dafny_input):
+def aws_cryptography_keystore_DeleteMutationOutput(dafny_input):
     return (
-        aws_cryptographic_materialproviders.smithygenerated.aws_cryptography_keystore.models.DeleteMutationLockAndIndexOutput()
+        aws_cryptographic_materialproviders.smithygenerated.aws_cryptography_keystore.models.DeleteMutationOutput()
     )
 
 
