AwsCryptographicMaterialProviders/runtimes/python/src/aws_cryptographic_materialproviders/smithygenerated/aws_cryptography_keystore/deserialize.py
@@ -11,7 +11,7 @@ from aws_cryptographic_materialproviders.internaldafny.generated.AwsCryptography
     Error_KeyManagementException,
     Error_KeyStorageException,
     Error_KeyStoreException,
-    Error_MutationLockConditionFailed,
+    Error_MutationCommitmentConditionFailed,
     Error_NoLongerExistsConditionFailed,
     Error_OldEncConditionFailed,
     Error_VersionRaceException,
@@ -34,7 +34,7 @@ from .errors import (
     KeyManagementException,
     KeyStorageException,
     KeyStoreException,
-    MutationLockConditionFailed,
+    MutationCommitmentConditionFailed,
     NoLongerExistsConditionFailed,
     OldEncConditionFailed,
     OpaqueError,
@@ -130,8 +130,10 @@ def _deserialize_error(error: Error) -> ServiceError:
         return KeyStorageException(message=_dafny.string_of(error.message))
     elif error.is_KeyStoreException:
         return KeyStoreException(message=_dafny.string_of(error.message))
-    elif error.is_MutationLockConditionFailed:
-        return MutationLockConditionFailed(message=_dafny.string_of(error.message))
+    elif error.is_MutationCommitmentConditionFailed:
+        return MutationCommitmentConditionFailed(
+            message=_dafny.string_of(error.message)
+        )
     elif error.is_NoLongerExistsConditionFailed:
         return NoLongerExistsConditionFailed(message=_dafny.string_of(error.message))
     elif error.is_OldEncConditionFailed:
